LaxLogic.lean
@@ -1,3 +1,10 @@
 -- This module serves as the root of the `LaxLogic` library.
 -- Import modules here that should be built as part of the library.
 import LaxLogic.PLLProof
+import LaxLogic.PLLNDCore
+import LaxLogic.PLLKripke
+import LaxLogic.PLLConsequence
+import LaxLogic.PLLCompleteness
+import LaxLogic.PLLTheorems
+import LaxLogic.PLLFrames
+import LaxLogic.PLLHilbert
